src/cddl/spec/CDDL.Spec.AST.Driver.fst
@@ -8,11 +8,24 @@ let print_endline (s: string) : ML unit =
   print_string s;
   print_newline ()
 
+unfold
+let ast_env_extend_typ_with_pre
+  (e: ast_env)
+  (new_name: string)
+  (t: typ)
+  (t_wf: ast0_wf_typ t)
+: GTot prop
+=
+    e.e_sem_env.se_bound new_name == None /\
+    typ_bounded e.e_sem_env.se_bound t /\
+    bounded_wf_typ (extend_name_env e.e_sem_env.se_bound new_name NType) t t_wf /\
+    spec_wf_typ (ast_env_extend_gen e new_name NType t).e_sem_env t t_wf
+
 let rec elab_list'
   (fuel: nat)
-  (env: wf_ast_env)
+  (env: ast_env)
   (l: list (string & typ))
-: ML (result wf_ast_env)
+: ML (result ast_env)
 = match l with
   | [] ->
     print_endline "Done, no definitions left";
@@ -26,7 +39,7 @@ let rec elab_list'
       print_endline "ERROR: Name already in use";
       RFailure (new_name ^ " already in use")
     | _ ->
-      let rec aux (fuel': nat) : ML (result wf_ast_env) =
+      let rec aux (fuel': nat) : ML (result ast_env) =
         let res = mk_wf_typ' fuel env t in
         print_endline "Result:";
         print_endline (ast0_wf_typ_result_to_string _ res);
@@ -39,8 +52,10 @@ let rec elab_list'
           aux (fuel' + fuel')
         | RSuccess t_wf ->
           print_endline "Success! Extending the environment";
-          assert (wf_ast_env_extend_typ_with_weak_pre' env new_name t t_wf); // FIXME: WHY WHY WHY?
-          let env' = wf_ast_env_extend_typ_with_weak env new_name t t_wf in
+          assert (bounded_wf_typ (env.e_sem_env.se_bound) t t_wf);
+          bounded_wf_typ_incr (env.e_sem_env.se_bound) (extend_name_env env.e_sem_env.se_bound new_name NType) t t_wf;
+          assert (ast_env_extend_typ_with_pre env new_name t t_wf); // FIXME: WHY WHY WHY?
+          let env' = ast_env_extend_typ_with env new_name t t_wf in
           elab_list' fuel' env' q
       in
       aux fuel
@@ -48,5 +63,5 @@ let rec elab_list'
 
 let elab_list
   (l: list (string & typ))
-: ML (result wf_ast_env)
+: ML (result ast_env)
 = elab_list' 0 empty_ast_env l
